ST_Abs WIP (problematic interp definition)

soundness.v
@@ -5,9 +5,9 @@ From Equations Require Import Equations.
 
 Definition γ_ok Γ γ0 γ1 := forall i, i < length Γ -> forall m PA, InterpUnivN m (subst_tm γ0 (dep_ith Γ i)) (subst_tm γ1 (dep_ith Γ i)) PA -> PA (γ0 i) (γ1 i).
 
-Definition SemWt Γ a b A B := forall γ0 γ1, γ_ok Γ γ0 γ1 -> exists m PA, InterpUnivN m (subst_tm γ0 A) (subst_tm γ1 B) PA /\ PA (subst_tm γ0 a) (subst_tm γ1 b).
+Definition SemWt Γ a A := forall γ0 γ1, γ_ok Γ γ0 γ1 -> exists m PA, InterpUnivN m (subst_tm γ0 A) (subst_tm γ1 A) PA /\ PA (subst_tm γ0 a) (subst_tm γ1 a).
 
-Definition SemWff Γ := forall i, i < length Γ -> exists F, SemWt (skipn (S i) Γ) (ith Γ i) (ith Γ i) (tUniv (F i)) (tUniv (F i)).
+Definition SemWff Γ := forall i, i < length Γ -> exists F, SemWt (skipn (S i) Γ) (ith Γ i) (tUniv (F i)).
 
 Lemma γ_ok_cons {i Γ γ0 γ1 a b PA A B} :
   InterpUnivN i (subst_tm γ0 A) (subst_tm γ1 B) PA ->
@@ -45,11 +45,11 @@ Proof.
   by apply h1; lia.
 Qed.
 
-Lemma renaming_SemWt Γ a b A B :
-  SemWt Γ a b A B ->
+Lemma renaming_SemWt Γ a A :
+  SemWt Γ a A ->
   forall Δ ξ,
     good_renaming ξ Γ Δ ->
-    SemWt Δ (ren_tm ξ a) (ren_tm ξ b) (ren_tm ξ A) (ren_tm ξ B).
+    SemWt Δ (ren_tm ξ a) (ren_tm ξ A).
 Proof.
   rewrite /SemWt => h Δ ξ hξ γ0 γ1 hγ.
   have hγ' : (γ_ok Γ (ξ >> γ0) (ξ >> γ1)) by eauto using γ_ok_renaming.
@@ -78,12 +78,12 @@ Section SemanticTyping.
     SemWff Γ ->
     i < length Γ ->
     (* ----------------------------------------------------- *)
-    SemWt Γ (var_tm i) (var_tm i) (dep_ith Γ i) (dep_ith Γ i).
+    SemWt Γ (var_tm i) (dep_ith Γ i).
   Proof using Γ.
     move => ih ? γ0 γ1 hγ.
     move /(_ i ltac:(done)) in ih.
     case : ih => F ih.
-    suff ih' : SemWt Γ (dep_ith Γ i) (dep_ith Γ i) (tUniv (F i)) (tUniv (F i)).
+    suff ih' : SemWt Γ (dep_ith Γ i) (tUniv (F i)).
     + case /(_ _ _ hγ) : ih' => j [PA [hPA hi]].
       simpl in hPA.
       case /InterpUnivN_Univ_inv' : hPA => ? ?; subst.
@@ -94,16 +94,51 @@ Section SemanticTyping.
 
   Lemma ST_False :
     SemWff Γ ->
-    SemWt Γ tFalse tFalse (tUniv m) (tUniv m).
+    SemWt Γ tFalse (tUniv m).
   Proof using m.
     hauto l:on use:InterpUniv_Univ, InterpUniv_False.
   Qed.
 
-  Lemma ST_Pi :
-    SemWt Γ (tPi A B) (tPi A B) (tUniv m) (tUniv m) ->
+  Lemma ST_Abs :
+    SemWt Γ (tPi A B) (tUniv m) ->
     SemWt (A :: Γ) a B ->
     (* ----------------------- *)
-    SemWt (tAbs )
+    SemWt Γ (tAbs A a) (tPi A B).
+  Proof.
+    rewrite /SemWt.
+    move => //  h0 h1 γ0 γ1 hγ.
+    move /(_ γ0 γ1 hγ) : h0; intros (n & P_Univ & hP_Univ & hP_Univ').
+    move /InterpUnivN_Univ_inv' : hP_Univ => [*]; subst.
+    case : hP_Univ' => PA hPA.
+    exists m, PA; split; first by auto.
+    simpl in hPA.
+    move /InterpUniv_Fun_inv : hPA.
+    rename PA into PA0.
+    intros (A0 & B0 & PA & PF & ? & hPA0 & hTot & hRes & hPF & ?). subst.
+    move => a0 a1 PB ha hPB.
+    move /InterpUniv_Refl in hPA0.
+    have hγ' : γ_ok (subst_tm γ0 A :: Γ) (a0 .: γ0) (a1 .: γ1) by
+    apply : γ_ok_cons ;eauto.
+    simpl.
+    apply : InterpUnivN_back_clos; eauto.
+
+
+    move /InterpUnivN_inv_Fun : hPA .
+    exists (S m), (fun A B => exists PA, InterpUnivN m A B PA).
+    split; first by best use: InterpUnivN_Univ_inv.
+    exists (ProdSpace PA (fun a PB => InterpUnivN i (subst_tm (a .: γ) B) PB)).
+    simp InterpUniv.
+    simpl.
+    apply InterpExt_Fun.
+    + simp InterpUniv in hPA.
+    + move => a ha.
+      move /(_ _ ltac:(qauto use:γ_ok_consU)) in h1.
+      move : h1; intros (x & PB & hPB & h).
+      move /InterpUnivN_Univ_inv' : hPB => [*]; subst.
+      hauto lq:on rew:db:InterpUniv.
+    + move => a PB ha.
+      suff hγ_cons : γ_ok (A :: Γ) (a .: γ) by asimpl.
+      qauto use:γ_ok_consU.
 
 End SemanticTyping.
 
@@ -113,20 +148,8 @@ Theorem soundness Γ :
 Proof.
   move : Γ.
   apply wt_mutual.
-  - move => Γ i h ih ? γ hγ.
-    move /(_ i ltac:(done)) in ih.
-    case : ih => F ih.
-    suff ih' : SemWt Γ (dep_ith Γ i) (tUniv (F i)).
-    + case /(_ _ hγ) : ih' => j [PA [hPA hi]].
-      simpl in hPA.
-      simp InterpUniv in hPA.
-      move /InterpExt_Univ_inv : hPA => [? h0]; subst.
-      move : hi; intros (PA & hi).
-      exists (F i), PA; sfirstorder.
-    + hauto l:on use:dep_ith_shift, good_renaming_truncate, renaming_SemWt.
-  - move => Γ i γ hγ.
-    exists (S i), (fun A => exists PA, InterpUnivN i A PA).
-    hauto l:on use:InterpUnivN_Univ_inv.
+  -
+  -
   - rewrite /SemWt.
     move => // Γ i A B _h0 h0 _h1 h1 γ hγ.
     move /(_ γ hγ) : h0; intros (m & P_Univ & hP_Univ & hP_Univ').
